

V4A9 Homework 10

So Murata, Heijing Shi

WiSe 25/26, University of Bonn Number Theory 1

1.
(a)

$$F : \text{Hom}_G(V, \widetilde{W}) \ni f \mapsto [W \ni w \mapsto (v \mapsto (f(v)(w)))].$$

We check the smoothness, that is

$$\tilde{\pi}(g)(F(f))(w) = \tilde{\pi}(g)(v \mapsto f(v)(w)) = (v \mapsto f(\pi(g^{-1})(v))(w)) = (v \mapsto f(v)(\sigma(g)(w))).$$

For the G -equivariance, set $\Phi = F(f)$,

$$\begin{aligned} \Phi(\sigma(g)w) &= (v \mapsto f(v)(\sigma(g)w)), \\ &= (v \mapsto (\tilde{\sigma}(g^{-1})f(v))(w)), \\ &= (v \mapsto (f(\pi(g^{-1})(v))(w))), \\ &= \tilde{\pi}(g)(v \mapsto f(v)(w)), \\ &= \tilde{\pi}(g)\Phi(w). \end{aligned}$$

We then construct a similar map $G : \text{Hom}_G(W, \tilde{V}) \rightarrow \text{Hom}_G(V, \tilde{W})$.

(b)

$$\begin{aligned} \text{Hom}_P(\pi, \rho_U(\tilde{\sigma})) &\cong \text{Hom}_G(i_P^G(\pi), \tilde{\sigma}), \\ &\stackrel{\text{(a)}}{\cong} \text{Hom}(\sigma, i_P^G(\tilde{\pi})), \\ &\stackrel{\text{HW9.3}}{\cong} \text{Hom}(\sigma, i_P^G(\tilde{\pi})), \\ &\cong \text{Hom}_L(\rho_U(\sigma), \tilde{\pi}), \\ &\cong \text{Hom}_L(\pi, \rho_U(\tilde{\sigma})). \end{aligned}$$

Using Yoneda Lemma, we have the isomorphism.

2. Suppose we have the result in **1**,

$$\begin{aligned} \text{Hom}_G(i_P^G(\sigma), \tilde{\pi}) &= \text{Hom}_G(\pi, i_P^G(\tilde{\sigma})), \\ &= \text{Hom}_G(\pi, i_P^G(\tilde{\sigma})), \\ &= \text{Hom}_L(\rho_U(\pi), \tilde{\sigma}), \\ &= \text{Hom}_L(\rho_U(\pi), \tilde{\sigma}), \\ &= \text{Hom}_L(\sigma, \rho_U(\tilde{\pi})). \end{aligned}$$

We have a injection $\pi \hookrightarrow \tilde{\pi}$. Set $\pi_1 = \text{coker}(\pi \hookrightarrow \tilde{\pi})$, then the second adjunction holds for $\tilde{\pi}$ and $\tilde{\pi}_1$. Considering the exact sequence,

$$0 \longrightarrow \pi \hookrightarrow \tilde{\pi} \longrightarrow \tilde{\pi}_1$$

By the naturality we have the second adjunction holds for $\ker f = \pi$. The last arrow is the composition of

$$\tilde{\pi} \longrightarrow \pi_1 \hookrightarrow \tilde{\pi}_1$$

As $\pi_1 \rightarrow \tilde{\pi}_1$ is injective it preserves the kernel.

$$\begin{array}{ccccc} 0 & \longrightarrow & \text{Hom}_G(i_P^G(\sigma), \pi) & \longrightarrow & \text{Hom}_G(i_P^G(\sigma), \tilde{\pi}) \xrightarrow{f_1} \text{Hom}_G(i_P^G(\sigma), \tilde{\pi}_1) \\ & & \vdots & & \downarrow \sim \\ 0 & \longrightarrow & \text{Hom}_L(\sigma, \rho_{\overline{U}}(\pi)) & \longrightarrow & \text{Hom}_L(\sigma, \rho_{\overline{U}}(\tilde{\pi})) \xrightarrow{f_2} \text{Hom}_L(\sigma, \rho_U(\tilde{\pi}_1)) \end{array}$$

Note that $\text{Hom}_G(i_P^G(\sigma), \cdot)$ is left exact and $\rho_{\overline{U}}(\cdot)$ is exact, thus the composition of two left exact functors are still left-exact. Thus Φ induces $\ker f_1 \cong \ker f_2$.

3.

$$\begin{aligned} t_p(b) &= i_P^G(b), \\ V_{\text{Ind}_P^G(\Sigma)} &\mapsto V_\Sigma, \\ f &\mapsto f(1). \end{aligned}$$

Suppose $i_P^G(b) = 0$ then $b(f(g)) = 0 \forall g \in G$ where $f \in V_{\text{Ind}_P^G(\Sigma)}$. For $v \in V_\Sigma$, then take

$$a_v : G \rightarrow V_\Sigma, g \mapsto \begin{cases} \Sigma(p)v, & (g = pk \in PK_0), \\ 0, & (\text{otherwise}) \end{cases}$$

Σ is smooth as of $(V_\Sigma)^K$ for same open compact $K \subseteq P$, such that $K \supset K_0 \cap P$.

4. Let

$$\Sigma_1 = \text{c-ind}_{H'}^H(\sigma) \otimes (\delta_G/\delta_H)^{-1}, \Sigma_2 = \text{c-ind}_{H'}^H(\sigma) \otimes (\delta(G)/\delta(H'))^{-1}.$$

$$\text{c-ind}_H^G(\text{c-ind}_{H'}^H(\sigma)) = \text{c-ind}_H^G(\Sigma_1 \otimes (\delta_G/\delta_H)) \longleftarrow \mathcal{H}(G) \otimes_{\mathcal{H}(H)} \Sigma_1$$

$$\Sigma_1 = \text{c-ind}_{H'}^H(\Sigma_2 \otimes (\delta_G/\delta_H)) \longleftarrow \mathcal{H}(H) \otimes_{\mathcal{H}(H')} \Sigma_2$$

$$\begin{aligned} \mathcal{H}(G) \otimes_{\mathcal{H}(H)} \Sigma_1 &= \mathcal{H}(G) \otimes_{\mathcal{H}(H)} (\mathcal{H}(H) \otimes_{\mathcal{H}(H')} \Sigma_2) \xrightarrow{\cong} \mathcal{H}(G) \otimes_{\mathcal{H}(H')} \Sigma_2 \\ &\quad \updownarrow \\ &\quad \text{c-ind}_{H'}^G(\Sigma_2 \otimes (\delta_G/\delta_{H'})) \end{aligned}$$

Recall we have,

$$\mathrm{c}\text{-ind}_H^G(\mathrm{c}\text{-ind}_{H'}^G(\sigma \otimes_1 / \delta_{H'})) \cong \mathrm{c}\text{-ind}_H^G(\mathrm{c}\text{-ind}_{H'}^H(\sigma \otimes (\delta_H / \delta_{H'})) \otimes_1 / \delta_H) \cong \mathrm{c}\text{-ind}_{H'}^G(\sigma \otimes_1 / \delta_{H'}).$$